wip

fstar-helpers/minicore/src/fstar_utils.rs
@@ -1,0 +1,23 @@
+pub mod manual_norm {
+    /// An F* stuck term that blocks normalization.
+    #[hax_lib::fstar::before("irreducible")]
+    pub const MANUAL_NORM: () = ();
+
+    /// A lemma that normalizes `MANUAL_NORM` away.
+    #[hax_lib::lemma]
+    pub fn manual_norm_lemma(_: ()) -> Proof<{ hax_lib::eq(MANUAL_NORM, ()) }> {}
+
+    /// Makes an expression opaque to the F* normalizer.
+    #[macro_export]
+    macro_rules! opaque {
+        (|$($x:ident : $ty:ty),*| -> $out:ty {$body:expr}) => {{
+            #[hax_lib::fstar::before("[@@strict_on_arguments [0]]")]
+            fn leaf(_: (), $($x:$ty,)*) -> $out {
+                $body
+            }
+            (|$($x:$ty,)*| leaf(MANUAL_NORM, $($x)*))
+        }};
+    }
+    pub use opaque;
+}
+pub use manual_norm::*;
